examples/dev/sw/interface.sml
@@ -1,11 +1,9 @@
 structure interface = struct
 
-  structure IR = annotatedIL
-
   val compile_ir =  funCall.link_ir
-  val sfl2ir = IR.sfl2ir
-  val printIR = IR.printIR
-  val printIR2 = IR.printIR2
+  val sfl2ir = annotatedIL.sfl2ir
+  val printIR = annotatedIL.printIR
+  val printIR2 = annotatedIL.printIR2
 
 (*
   val pp_compile = pp_compile;
